fstar/XXX.fst
@@ -1,0 +1,100 @@
+module XXX
+
+open FStar.Tactics
+open Hacspec.Lib
+open FStar.Mul
+open Hacspec.Chacha20
+
+module S = Spec.Chacha20
+module H = Hacspec.Chacha20
+module Seq = Lib.Sequence
+
+module LC = Lib.LoopCombinators
+
+#set-options "--fuel 0 --ifuel 0 --z3rlimit 30"
+
+let rec foldi
+  (lo: uint_size)
+  (hi: uint_size{lo <= hi})
+  (f: (i:uint_size{i < hi}) -> 'a -> 'a)
+  (init: 'a)
+  : Tot 'a (decreases (hi - lo))
+  = if lo = hi then init
+               else foldi (lo+1) hi f (f lo init)
+
+unfold let map_blocks_foldi
+    (#len: uint_size) (blocksize: size_pos)
+    (max: uint_size {max * blocksize <= len})
+    (n: uint_size {n * blocksize <= len /\ n <= max})
+    (original_s: lseq 'a len)
+    (s: lseq 'a len)
+    (f:(i:nat{i < max}) -> lseq 'a blocksize -> lseq 'a blocksize)
+    : lseq 'a len
+  = foldi #(lseq 'a len) 0 n (fun (i: nat{i<max}) (s: lseq 'a len) -> seq_set_exact_chunk #'a #len s blocksize i (f i (seq_get_exact_chunk #'a original_s blocksize i))) s
+
+#push-options "--print_implicits --print_universes"
+
+let manual_rewrite (): Lemma (uint8 == int_t U8 SEC) = ()
+
+
+// let seq_set_exact_chunk
+//   (#a: Type)
+//   (#len:uint_size) (* change to nseq but update_sub missing for nseq *)
+//   (s: lseq a len)
+//   (chunk_len: uint_size)
+//   (chunk_num: uint_size)
+//   (chunk: seq a )
+//     : Pure (lseq a len)
+//       (requires (
+//         chunk_len * (chunk_num + 1) <= FStar.Seq.length s /\
+//         Seq.length chunk = seq_chunk_len s chunk_len chunk_num
+//       ))
+//       (ensures (fun out -> True))
+//   = s
+
+
+let chacha20_update0' (st0 : state_t) (cipher : byte_seq) =
+  let blocks_out: seq uint8 = seq_new_ (secret (pub_u8 0x0)) (seq_len cipher) in
+  let n_blocks: uint_size = seq_num_exact_chunks cipher 64 in
+    
+  let rr = foldi #(lseq (int_t U8 SEC) (seq_len #(int_t U8 SEC) cipher))
+          0
+          (seq_num_exact_chunks #(int_t U8 SEC) cipher 64)
+          (fun i s ->
+              seq_set_exact_chunk #(int_t U8 SEC)
+                #(seq_len #(int_t U8 SEC) cipher)
+                s
+                64
+                i
+                (chacha20_encrypt_block st0
+                    (secret #U32 (pub_u32 i))
+                    (array_from_seq #(int_t U8 SEC)
+                        64
+                        (seq_get_exact_chunk #(int_t U8 SEC) cipher 64 i))
+                  <:
+                  Prims.Tot block_t))
+          (seq_new_ #(int_t U8 SEC) (secret #U8 (pub_u8 0x0)) (seq_len #(int_t U8 SEC) cipher)) in
+
+  let f2 (i: nat {i<n_blocks}) (msg_block: lseq uint8 64): block_t = 
+    chacha20_encrypt_block st0 (secret (pub_u32 i)) (array_from_seq 64 msg_block)
+  in
+  let r2 = map_blocks_foldi #uint8 #(seq_len cipher) 64 n_blocks n_blocks cipher blocks_out f2 in
+
+  assert (eq2 #(seq _) r2 rr) by (
+    norm [delta_only [`%map_blocks_foldi;`%uint8;`%uint_t;`%lseq;`%seq_len]; zeta_full];
+    norm [unascribe];
+    norm [delta_only [`%Seq.lseq;`%seq_len]];
+    l_to_r [`manual_rewrite];
+    let goal = cur_goal () in
+    let _squash, [goal,_] = admit (); collect_app goal in
+    let _eq2, [_;(l,_);(r,_)] = admit (); collect_app goal in
+    print ("lllllllllllllllll");
+    print (term_to_string l);
+    print ("rrrrrrrrrrrrrrrrr");
+    print (term_to_string r);
+    // if compare_term l r = FStar.Order.Eq
+    // then fail "hey";
+    // trefl ();
+    fail "x"
+  );
+  admit ()
